src/Bedrock/Group/ScalarMult/LadderStep.v
@@ -1,11 +1,14 @@
 Require Import Rupicola.Lib.Api. Import bedrock2.WeakestPrecondition.
 Require Import Crypto.Arithmetic.PrimeFieldTheorems.
-Require Import Crypto.Bedrock.Specs.Field.
+Require Import Crypto.Bedrock.Specs.AbstractField.
+Require Import Crypto.Bedrock.Specs.PrimeField.
 Require Import Crypto.Bedrock.Field.Interface.Compilation2.
 Local Open Scope Z_scope.
 
 Section Gallina.
   Local Open Scope F_scope.
+
+  Let F := F.F.
 
   Definition ladderstep_gallina (m : positive) (a24 : F m)
              (X1 X2 Z2 X3 Z3: F m) : \<< F m, F m, F m, F m \>> :=
@@ -39,11 +42,17 @@ Section __.
   Context {locals_ok : map.ok locals}.
   Context {env_ok : map.ok env}.
   Context {ext_spec_ok : Semantics.ext_spec.ok ext_spec}.
-  Context {field_parameters : FieldParameters}
-          {field_representaton : FieldRepresentation}
+  Context {prime_field_parameters : PrimeFieldParameters}.
+
+  Instance my_field_parameters : FieldParameters := PrimeField.prime_field_parameters.
+  
+  Context {field_representaton : FieldRepresentation}
           {field_representation_ok : FieldRepresentation_ok}.
+
   Hint Resolve relax_bounds : compiler.
   Existing Instance felem_alloc.
+
+  Let F := F.F.
 
   Instance spec_of_ladderstep : spec_of "ladderstep" :=
     fnspec! "ladderstep"
@@ -124,14 +133,155 @@ Section __.
   Qed.
 
   Local Ltac ecancel_assumption ::=  ecancel_assumption_impl.
+
+  (*Why must these instances be included?*)
+
+  Instance spec_of_mul : spec_of (@mul prime_field_parameters).
+  Proof.
+    pose proof (binop_spec bin_mul). cbv [spec_of]. eapply X.
+  Defined.
+
+  Instance spec_of_square : spec_of (@square prime_field_parameters).
+  Proof.
+    pose proof (unop_spec un_square). cbv [spec_of]. eapply X.
+  Defined.
+
+  Instance spec_of_add : spec_of (@add prime_field_parameters).
+  Proof.
+    pose proof (binop_spec bin_add). cbv [spec_of]. eapply X.
+  Defined.
+
+  Instance spec_of_sub : spec_of (@sub prime_field_parameters).
+  Proof.
+    pose proof (binop_spec bin_sub). cbv [spec_of]. eapply X.
+  Defined.
+
+  Instance spec_of_scmula24 : spec_of (@scmula24 prime_field_parameters).
+  Proof.
+    pose proof (unop_spec un_scmula24). cbv [spec_of]. eapply X.
+  Defined.
+
+  Lemma relax_bounds_FElem_R : forall R x x_ptr, Lift1Prop.impl1 ((FElem (Some tight_bounds) x_ptr x * R)%sep) ((FElem (Some loose_bounds) x_ptr x * R)%sep).
+  Proof.
+    intros. cbv [Lift1Prop.impl1]. intros.
+    destruct H, H, H, H0.
+    eexists; eexists; split; [eapply H | ]. split; eauto. eapply relax_bounds_FElem. auto.
+  Qed.
+
+  Lemma relax_bounds_binop : forall R x x_ptr y y_ptr, Lift1Prop.impl1 ((FElem (Some tight_bounds) x_ptr x * FElem (Some tight_bounds) y_ptr y * R)%sep) ((FElem (Some loose_bounds) x_ptr x * FElem (Some loose_bounds) y_ptr y * R)%sep).
+  Proof.
+    intros. cbv [Lift1Prop.impl1]. intros. eapply sep_assoc. eapply relax_bounds_FElem_R.
+    eapply sep_comm, sep_assoc. eapply relax_bounds_FElem_R. ecancel_assumption.
+  Qed.
+
+  (*tactics for applying field operations*)
+
+  Ltac find_in_map :=
+    repeat first [ erewrite map.get_put_diff; [| intros contra; discriminate] |
+      eapply map.get_put_same].
+
+  Ltac apply_square :=
+      try simple apply compile_nlet_as_nlet_eq;
+      epose proof compile_square as Hsquare;
+      cbv [AbstractField.F] in Hsquare; cbv [Compilation2.field_parameters PrimeField.prime_field_parameters] in *;
+      cbv [AbstractField.square AbstractField.Fsquare Fmul Compilation2.field_parameters] in *;
+      rewrite F.pow_2_r;
+      eapply Hsquare; clear Hsquare; try repeat compile_step; [ eapply relax_bounds_FElem_R; ecancel_assumption | ..]; repeat compile_step.
+
+      
+  Ltac apply_mul :=
+    try simple apply compile_nlet_as_nlet_eq;
+    epose proof compile_mul as Hmul;
+    cbv [AbstractField.F] in Hmul; cbv [Compilation2.field_parameters PrimeField.prime_field_parameters] in *;
+    cbv [AbstractField.mul AbstractField.Fmul Fmul Compilation2.field_parameters] in *;
+    eapply Hmul; clear Hmul; try repeat compile_step; [ eapply sep_assoc, relax_bounds_FElem_R, sep_comm, sep_assoc, relax_bounds_FElem_R; ecancel_assumption | compile_step| compile_step| ..]. 
   
+  Ltac apply_add :=
+    try simple apply compile_nlet_as_nlet_eq;
+    epose proof compile_add as Hadd;
+    cbv [AbstractField.F] in Hadd; cbv [Compilation2.field_parameters PrimeField.prime_field_parameters] in *;
+    cbv [AbstractField.add AbstractField.Fadd Fadd Compilation2.field_parameters] in *;
+    eapply Hadd; clear Hadd; [| find_in_map | eapply relax_bounds_FElem_R; ecancel_assumption| ecancel_assumption| ..]; try compile_step.
+
+  Ltac apply_sub :=
+    try simple apply compile_nlet_as_nlet_eq;
+    epose proof compile_sub as Hsub;
+    cbv [AbstractField.F] in Hsub; cbv [Compilation2.field_parameters PrimeField.prime_field_parameters] in *;
+    cbv [AbstractField.sub AbstractField.Fsub Fsub Compilation2.field_parameters] in *;
+    eapply Hsub; clear Hsub; [| find_in_map | eapply relax_bounds_FElem_R; ecancel_assumption| ecancel_assumption| ..]; try compile_step.
+    
+
+  Local Hint Extern 8 (WeakestPrecondition.cmd _ _ _ _ _ (_ (nlet_eq _ (_ ^ 2)%F _))) =>
+    let Hsquare := (fresh "Hsquare") in pose proof compile_square as Hsquare;
+    rewrite F.pow_2_r; cbv [Compilation2.field_parameters PrimeField.prime_field_parameters] in Hsquare;
+    eapply Hsquare; clear Hsquare; shelve : compiler.
+
+    Local Hint Extern 6 (WeakestPrecondition.cmd _ _ _ _ _ (_ (nlet_eq _ (a24 * _)%F _))) =>
+    let Hscmul := (fresh "Hscmul") in epose proof compile_scmula24 as Hscmul;
+    cbv [Compilation2.field_parameters PrimeField.prime_field_parameters] in *;
+    eapply Hscmul; clear Hscmul; shelve : compiler.
+
+  Local Hint Extern 8 (WeakestPrecondition.cmd _ _ _ _ _ (_ (nlet_eq _ (_ * _)%F _))) =>
+    let Hmul := (fresh "Hmul") in pose proof compile_mul as Hmul;
+    cbv [Compilation2.field_parameters PrimeField.prime_field_parameters] in Hmul;
+    eapply Hmul; [| | | try (eapply relax_bounds_binop; ecancel_assumption) | | |]; clear Hmul; shelve : compiler.
+
+    Local Hint Extern 8 (WeakestPrecondition.cmd _ _ _ _ _ (_ (nlet_eq _ (_ - _)%F _))) =>
+    let Hsub := (fresh "Hsub") in epose proof compile_sub as Hsub;
+    cbv [Compilation2.field_parameters PrimeField.prime_field_parameters] in *;
+    eapply Hsub; clear Hsub; shelve : compiler.
+
+  Local Hint Extern 8 (WeakestPrecondition.cmd _ _ _ _ _ (_ (nlet_eq _ (_ + _)%F _))) =>
+    let Hadd := (fresh "Hadd") in epose proof compile_add as Hadd;
+    cbv [Compilation2.field_parameters PrimeField.prime_field_parameters] in *;
+    eapply Hadd; clear Hadd; shelve : compiler.
+
+  Local Hint Extern 9 ((FElem (Some loose_bounds) _ _ ⋆ FElem (Some loose_bounds) _ _ ⋆ _)%sep _) =>
+    eapply relax_bounds_binop; ecancel_assumption : compiler.
+
+  Local Hint Extern 9 =>
+  simple eapply (@compile_stack _ _ _ _ _ _ _ _ _ _ _ _ _ _ _ _ _ _ _ _ _ _
+    ((@FElem width BW word mem prime_field_parameters field_representaton
+    (@None (@bounds field_parameters width BW word mem field_representaton)))));
+    [ecancel_assumption | shelve] : compiler.
+
+
+  Lemma FElem_bounds_None : forall x x_ptr R, Lift1Prop.impl1 (FElem (Some loose_bounds) x_ptr x * R)%sep (FElem None x_ptr x * R)%sep.
+  Proof.
+    intros. cbv [Lift1Prop.impl1]; intros m Hsep.
+    destruct Hsep as [m1 [m2 [Hsep1 [Hsep2 Hsep3]]]].
+    do 2 eexists. split; eauto. split; eauto.
+    cbv [FElem Lift1Prop.ex1] in *. sepsimpl. simpl.
+    exists x0. sepsimpl; auto.
+  Qed.
+
+  Local Hint Extern 9 ((FElem None _ _ ⋆ _ )%sep _) =>
+  eapply FElem_bounds_None; ecancel_assumption : compiler_cleanup_post.
+
+  Ltac clear_pred_seps' :=   
+  unfold pred_sep;
+  repeat change (fun x => ?h x) with h;
+  repeat match goal with
+         | [ H : _ ?m |- _ ?m] =>
+           eapply Proper_sep_impl1;
+           [ eapply P_to_bytes | clear H m; intros H m |
+            try (eapply FElem_bounds_None; ecancel_assumption);
+            try (eapply FElem_bounds_None; eapply relax_bounds_FElem_R; ecancel_assumption)]
+         end.
+
+  Hint Extern 1 (pred_sep _ _ _ _ _ _) =>
+         clear_pred_seps'; shelve : compiler_cleanup_post.
+
+
   Derive ladderstep_body SuchThat
          (defn! "ladderstep" ("X1", "X2", "Z2", "X3", "Z3")
               { ladderstep_body },
            implements ladderstep_gallina
-                      using [mul;add;sub;square;scmula24])
+                      using [@mul prime_field_parameters;@add prime_field_parameters;@sub prime_field_parameters;@square prime_field_parameters;@scmula24 prime_field_parameters])
          As ladderstep_correct.
-  Proof. compile. Qed.
+  Proof. 
+    compile.
+  Qed.
 
 End __.
 
