src/Bedrock/Specs/AbstractField.v
@@ -1,0 +1,291 @@
+Require Import coqutil.Byte.
+Require Import Rupicola.Lib.Api.
+Require Import Crypto.Algebra.Hierarchy.
+Require Import Crypto.Algebra.Field.
+Require Import Crypto.Bedrock.Field.Synthesis.Generic.Bignum.
+Require Import Crypto.Bedrock.Field.Common.Arrays.MaxBounds.
+Require Import Crypto.COperationSpecifications.
+Require Import Crypto.Util.ZUtil.ModInv.
+Local Open Scope Z_scope.
+Import bedrock2.Memory.
+
+Section FieldSpecs.
+
+  Class FieldParameters :=
+    { F : Type;
+      Fzero : F; Fone : F;
+      Feq : F -> F -> Prop;
+      Fopp : F -> F; Finv : F -> F;
+      Fadd : F -> F -> F; Fsub : F -> F -> F; Fmul : F -> F -> F; Fdiv : F -> F -> F; (*consider collecting these in a separate class.*)
+
+      Feq_dec : DecidableRel Feq;
+
+      a24 : F; (* (a+2) / 4 or (a-2) / 4, depending on the implementation *)
+
+      (* special wrapper for copy so that compilation lemmas can recognize it *)
+      fe_copy := (@id (F));
+
+      (** function names **)
+      mul : string; add : string; sub : string; opp : string;
+      square : string; scmula24 : string; inv : string;
+      from_bytes : string; to_bytes : string;
+      select_znz : string;
+
+      (* felem_small_literal p x :=
+          store p (expr.literal x);
+          store (p+4) (expr.literal 0);
+          ...
+
+        felem_copy pX pY :=
+          store pX (load pY);
+          store (pX+4) (load (pY+4));
+          ... *)
+      felem_copy : string;
+      from_word : string;
+    }.
+
+  Class FieldParameters_ok {field_parameters : FieldParameters} := {
+    fld:@Hierarchy.field F Feq Fzero Fone Fopp Fadd Fsub Fmul Finv Fdiv
+  }.
+
+  Class FieldRepresentation
+        {field_parameters : FieldParameters}
+        {width: Z} {BW: Bitwidth width} {word: word.word width} {mem: map.map word Byte.byte}
+        :=
+    { felem := list word;
+      feval : felem -> F;
+
+      feval_bytes : list byte -> F;
+      felem_size_in_words : nat;
+      felem_size_in_bytes : Z := Z.of_nat felem_size_in_words * bytes_per_word width; (* for stack allocation *)
+      encoded_felem_size_in_bytes : nat; (* number of bytes when serialized *)
+      bytes_in_bounds : list byte -> Prop;
+
+      (* Memory layout *)
+      FElem : word -> list word -> mem -> Prop := Bignum felem_size_in_words;
+      FElemBytes : word -> list byte -> mem -> Prop :=
+        fun addr bs =>
+          (emp (length bs = encoded_felem_size_in_bytes
+                /\ bytes_in_bounds bs)
+          * array ptsto (word.of_Z 1) addr bs)%sep;
+
+      bounds : Type;
+      bounded_by : bounds -> felem -> Prop;
+      (* for saturated implementations, loose/tight bounds are the same *)
+      loose_bounds : bounds;
+      tight_bounds : bounds;
+    }.
+
+  Definition Placeholder
+            {field_parameters : FieldParameters}
+            {width: Z} {BW: Bitwidth width} {word: word.word width} {mem: map.map word Byte.byte}
+            {field_representation : FieldRepresentation(mem:=mem)}
+            (p : word) : mem -> Prop :=
+    Memory.anybytes(mem:=mem) p felem_size_in_bytes.
+
+  Class FieldRepresentation_ok
+        {field_parameters : FieldParameters}
+        {width: Z} {BW: Bitwidth width} {word: word.word width} {mem: map.map word Byte.byte}
+        {field_representation : FieldRepresentation} := {
+      relax_bounds :
+        forall X : felem, bounded_by tight_bounds X
+                          -> bounded_by loose_bounds X;
+    }.
+
+  Section BignumToFieldRepresentationAdapterLemmas.
+    Context
+    {field_parameters : FieldParameters}
+    {width: Z} {BW: Bitwidth width} {word: word.word width} {mem: map.map word Byte.byte}
+    {field_representation : FieldRepresentation}.
+    Context {word_ok : @word.ok width word} {map_ok : @map.ok word Init.Byte.byte mem}.
+
+    Lemma felem_size_in_bytes_mod :
+          felem_size_in_bytes mod Memory.bytes_per_word width = 0.
+    Proof. apply Z_mod_mult. Qed.
+    Lemma FElem_from_bytes p : Lift1Prop.iff1 (Placeholder p) (Lift1Prop.ex1 (FElem p)).
+    Proof.
+      cbv [Placeholder FElem felem_size_in_bytes].
+      repeat intro.
+      cbv [Lift1Prop.ex1]; split; intros;
+        repeat match goal with
+              | H : anybytes _ _ _ |- _ => eapply Array.anybytes_to_array_1 in H
+              | H : exists _, _ |- _ => destruct H
+              | H : _ /\ _ |- _ => destruct H
+              end.
+        all : repeat match goal with
+              | H : anybytes _ _ _ |- _ => eapply Array.anybytes_to_array_1 in H
+              | H : exists _, _ |- _ => destruct H
+              | H : _ /\ _ |- _ => destruct H
+              end.
+      { eexists; eapply Bignum_of_bytes; try eassumption.
+        destruct Bitwidth.width_cases; subst width; revert H0; cbn; lia. }
+      { eapply Bignum_to_bytes in H; sepsimpl.
+        let H := match goal with
+                | H : Array.array _ _ _ _ _ |- _ => H end in
+        eapply Array.array_1_to_anybytes in H.
+        unshelve (erewrite (_:_*_=_); eassumption).
+        rewrite H; destruct Bitwidth.width_cases as [W|W];
+          symmetry in W; destruct W; cbn; clear; lia. }
+    Qed.
+  End BignumToFieldRepresentationAdapterLemmas.
+
+  Section ToFromBytes.
+    Definition nth_byte (x : Z) (n : nat) : byte :=
+      byte.of_Z (Z.shiftr x (8 * Z.of_nat n)).
+    Definition Z_to_bytes (x : Z) (n : nat) : list byte :=
+      List.map (nth_byte x) (seq 0 n).
+    Definition Z_from_bytes (bs : list byte) : Z :=
+      List.fold_right
+        (fun b acc => Z.shiftl acc 8 + byte.unsigned b) 0 bs.
+  End ToFromBytes.
+
+  Section FunctionSpecs.
+    Context {width: Z} {BW: Bitwidth width} {word: word.word width} {mem: map.map word Byte.byte}.
+    Context {locals: map.map String.string word}.
+    Context {env: map.map String.string (list String.string * list String.string * Syntax.cmd)}.
+    Context {ext_spec: bedrock2.Semantics.ExtSpec}.
+    Context {word_ok : word.ok word} {mem_ok : map.ok mem}.
+    Context {locals_ok : map.ok locals}.
+    Context {env_ok : map.ok env}.
+    Context {ext_spec_ok : Semantics.ext_spec.ok ext_spec}.
+    Context {field_parameters : FieldParameters}
+            {field_representation : FieldRepresentation}.
+
+    Local Definition Fsquare (x : F) := Fmul x x.
+
+    Class UnOp (name: string) :=
+      { un_model: F -> F;
+        un_xbounds: bounds;
+        un_outbounds: bounds }.
+
+    Import WeakestPrecondition.
+
+    Definition unop_spec {name} (op: UnOp name) :=
+      fnspec! name (pout px : word) / (out x : felem) Rr,
+      { requires tr mem :=
+          bounded_by un_xbounds x
+          /\ (exists Ra, (FElem px x * Ra)%sep mem)
+          /\ (FElem pout out * Rr)%sep mem;
+        ensures tr' mem' :=
+          tr = tr' /\
+          exists out,
+            feval out = un_model (feval x)
+            /\ bounded_by un_outbounds out
+            /\ (FElem pout out * Rr)%sep mem' }.
+
+    Instance spec_of_UnOp {name} (op: UnOp name) : spec_of name :=
+      unop_spec op.
+
+    Class BinOp (name: string) :=
+      { bin_model: F -> F -> F;
+        bin_xbounds: bounds;
+        bin_ybounds: bounds;
+        bin_outbounds: bounds }.
+
+    Definition binop_spec  {name} (op: BinOp name) :=
+      fnspec! name (pout px py : word) / (out x y : felem) Rr,
+      { requires tr mem :=
+          bounded_by bin_xbounds x
+          /\ bounded_by bin_ybounds y
+          /\ (exists Rx, (FElem px x * Rx)%sep mem)
+          /\ (exists Ry, (FElem py y * Ry)%sep mem)
+          /\ (FElem pout out * Rr)%sep mem;
+        ensures tr' mem' :=
+          tr = tr' /\
+          exists out,
+            feval out = bin_model (feval x) (feval y)
+            /\ bounded_by bin_outbounds out
+            /\ (FElem pout out * Rr)%sep mem' }.
+
+    Instance spec_of_BinOp {name} (op: BinOp name) : spec_of name :=
+      binop_spec op.
+
+    Instance bin_mul : BinOp mul :=
+      {| bin_model := Fmul; bin_xbounds := loose_bounds; bin_ybounds := loose_bounds; bin_outbounds := tight_bounds |}.
+    Instance un_square : UnOp square :=
+      {| un_model := fun x => Fsquare x; un_xbounds := loose_bounds; un_outbounds := tight_bounds |}.
+    Instance bin_add : BinOp add :=
+      {| bin_model := Fadd; bin_xbounds := tight_bounds; bin_ybounds := tight_bounds; bin_outbounds := loose_bounds |}.
+    Instance bin_sub : BinOp sub :=
+      {| bin_model := Fsub; bin_xbounds := tight_bounds; bin_ybounds := tight_bounds; bin_outbounds := loose_bounds |}.
+    Instance un_scmula24 : UnOp scmula24 :=
+      {| un_model := Fmul a24; un_xbounds := loose_bounds; un_outbounds := tight_bounds |}.
+    Instance un_inv : UnOp inv := (* TODO: what are the bounds for inv? *)
+      {| un_model := Finv; un_xbounds := tight_bounds; un_outbounds := loose_bounds |}.
+    Instance un_opp : UnOp opp :=
+      {| un_model := Fopp; un_xbounds := tight_bounds; un_outbounds := loose_bounds |}.
+
+    Instance spec_of_from_bytes : spec_of from_bytes :=
+      fnspec! from_bytes (pout px : word) / out (bs : list byte) Rr,
+      { requires tr mem :=
+          (exists Ra, (FElemBytes px bs * Ra)%sep mem)
+          /\ (FElem pout out * Rr)%sep mem;
+        ensures tr' mem' :=
+          tr = tr' /\
+          exists X, feval X = feval_bytes bs
+              /\ bounded_by tight_bounds X
+              /\ (FElem pout X * Rr)%sep mem' }.
+
+    Instance spec_of_to_bytes : spec_of to_bytes :=
+      fnspec! to_bytes (pout px : word) / (out : list byte) (x : felem) Rr,
+      { requires tr mem :=
+          bounded_by tight_bounds x /\
+          (exists Ra, (FElem px x * Ra)%sep mem)
+          /\ (FElemBytes pout out * Rr)%sep mem;
+        ensures tr' mem' :=
+          tr = tr' /\ 
+          exists bs,
+            feval x = feval_bytes bs /\
+            (FElemBytes pout bs * Rr)%sep mem' }.
+
+    Instance spec_of_felem_copy : spec_of felem_copy :=
+      fnspec! felem_copy (pout px : word) / (out x : felem) R,
+      { requires tr mem :=
+          (FElem px x * FElem pout out * R)%sep mem;
+        ensures tr' mem' :=
+          tr = tr' /\
+          (FElem px x * FElem pout x * R)%sep mem' }.
+
+      Local Notation bit_range := {|ZRange.lower := 0; ZRange.upper := 1|}.
+
+      Instance spec_of_selectznz  : spec_of select_znz :=
+      fnspec! select_znz (pout pc px py : word) / out Rout Rx Ry x y,
+      {
+          requires tr mem :=
+          (FElem pout out * Rout)%sep mem /\
+          (FElem px x * Rx)%sep mem /\
+          (FElem py y * Ry)%sep mem /\
+          ZRange.is_bounded_by_bool (word.unsigned pc) bit_range = true;
+          ensures tr' mem' :=
+          if ((word.unsigned pc) =? 1)
+              then ((FElem pout y * Rout)%sep mem')
+              else ((FElem pout x * Rout)%sep mem')
+      }.
+
+  End FunctionSpecs.
+
+  Existing Instances spec_of_UnOp spec_of_BinOp bin_mul un_square bin_add bin_sub
+          un_scmula24 un_inv spec_of_felem_copy.
+
+  Section SpecProperties.
+    Context {width: Z} {BW: Bitwidth width} {word: word.word width} {mem: map.map word Byte.byte}.
+    Context {locals: map.map String.string word}.
+    Context {env: map.map String.string (list String.string * list String.string * Syntax.cmd)}.
+    Context {ext_spec: bedrock2.Semantics.ExtSpec}.
+    Context {word_ok : word.ok word} {mem_ok : map.ok mem}.
+    Context {locals_ok : map.ok locals}.
+    Context {env_ok : map.ok env}.
+    Context {ext_spec_ok : Semantics.ext_spec.ok ext_spec}.
+    Context {field_parameters : FieldParameters}
+            {field_representation : FieldRepresentation}
+            {field_representation_ok : FieldRepresentation_ok}.
+
+    Lemma FElem_to_bytes px x :
+      Lift1Prop.impl1 (FElem px x) (Placeholder px).
+    Proof.
+      rewrite FElem_from_bytes.
+      repeat intro; eexists; eauto.
+    Qed.
+
+  End SpecProperties.
+End FieldSpecs.
