src/Bedrock/Specs/PrimeField.v
@@ -1,0 +1,111 @@
+Require Import Crypto.Bedrock.Specs.AbstractField.
+Require Import Crypto.Arithmetic.PrimeFieldTheorems.
+Require Import coqutil.Byte.
+Require Import Rupicola.Lib.Api.
+Require Import Crypto.Algebra.Hierarchy.
+Require Import Crypto.Arithmetic.PrimeFieldTheorems.
+Require Import Crypto.Bedrock.Field.Synthesis.Generic.Bignum.
+Require Import Crypto.Bedrock.Field.Common.Arrays.MaxBounds.
+Require Import Crypto.COperationSpecifications.
+Require Import Crypto.Util.ZUtil.ModInv.
+Local Open Scope Z_scope.
+Import bedrock2.Memory.
+
+Section PrimeField.
+
+Class PrimeFieldParameters :=
+  { (** mathematical parameters **)
+    M_pos : positive; (* modulus *)
+    M : Z := Z.pos M_pos;
+    a24 : F M_pos; (* (a+2) / 4 or (a-2) / 4, depending on the implementation *)
+
+    (* special wrapper for copy so that compilation lemmas can recognize it *)
+    fe_copy := (@id (F M_pos));
+
+    (** function names **)
+    mul : string; add : string; sub : string; opp : string;
+    square : string; scmula24 : string; inv : string;
+    from_bytes : string; to_bytes : string;
+    select_znz : string;
+
+    felem_copy : string;
+    from_word : string;
+  }.
+
+  Class PrimeFieldParameters_ok {field_parameters : PrimeFieldParameters} := {
+    M_prime : Znumtheory.prime M
+  }.
+
+  Section Specialized.
+    Context {params : PrimeFieldParameters}
+            {params_ok : @PrimeFieldParameters_ok params}
+            {width: Z} {BW: Bitwidth width} {word: word.word width} {mem: map.map word Byte.byte}.
+
+    Instance Field : (@field (F M_pos) (@eq (F M_pos)) (F.zero) (F.one) F.opp F.add F.sub F.mul F.inv F.div).
+    Proof.
+      exact (@F.field_modulo M_pos M_prime).
+    Defined.
+
+    Instance prime_field_parameters : FieldParameters.
+    Proof.
+      econstructor.
+        - exact (@F.zero M_pos).
+        - exact (@F.one M_pos).
+        - exact (@F.opp M_pos).
+        - exact (@F.inv M_pos).
+        - exact (@F.add M_pos).
+        - exact (@F.sub M_pos).
+        - exact (@F.mul M_pos).
+        - exact (@F.div M_pos).
+        - apply F.eq_dec.
+        - exact (a24).
+        - exact mul.
+        - exact add.
+        - exact sub.
+        - exact opp.
+        - exact square.
+        - exact scmula24.
+        - exact inv.
+        - exact from_bytes.
+        - exact to_bytes.
+        - exact select_znz.
+        - exact felem_copy.
+        - exact from_word.
+    Defined. 
+
+    Instance prime_field_parameters_ok : @AbstractField.FieldParameters_ok prime_field_parameters.
+    Proof.
+      constructor. apply Field.
+    Defined.
+
+    Context {locals : map.map string word}
+            {ext_spec : bedrock2.Semantics.ExtSpec}
+            {field_representation : FieldRepresentation}
+            {field_representation_ok : FieldRepresentation_ok}.
+      
+    Instance spec_of_from_word : spec_of from_word :=
+      fnspec! from_word (pout x : word) / out R,
+      { requires tr mem0 :=
+          (FElem pout out * R)%sep mem0;
+        ensures tr' mem' :=
+          tr = tr' /\
+          exists X, feval X = F.of_Z _ (word.unsigned x)
+              /\ bounded_by tight_bounds X
+              /\ (FElem pout X * R)%sep mem' }.
+
+    (* Parameters for word-by-word Montgomery arithmetic*)
+      Definition r := 2 ^ width.
+      Definition m' := Z.modinv (- M) r.
+      Definition r' := Z.modinv (r) M.
+    
+      Definition from_mont_model x := F.mul x (@F.of_Z M_pos (r' ^ (Z.of_nat felem_size_in_words)%Z)).
+      Definition to_mont_model x := F.mul x (@F.of_Z M_pos (r ^ (Z.of_nat felem_size_in_words)%Z)).
+    
+      Instance un_from_mont {from_mont : string} : UnOp from_mont :=
+        {| un_model := from_mont_model; un_xbounds := tight_bounds; un_outbounds := loose_bounds |}.
+    
+      Instance un_to_mont {to_mont : string} : UnOp to_mont :=
+        {| un_model := to_mont_model; un_xbounds := tight_bounds; un_outbounds := loose_bounds|}.
+
+  End Specialized.
+End PrimeField.
